progress on acquire

concurrency/framework/Cells.s.dfy
@@ -22,28 +22,28 @@ module {:extern "LinearCells"} LinearCells {
   import opened Options
 
   type {:extern "struct"} LinearCell(!new,00)<V>
-  datatype CellContents<V> = CellContents(ghost lcell: LinearCell<V>, v: Option<V>)
+  datatype LCellContents<V> = LCellContents(ghost lcell: LinearCell<V>, v: Option<V>)
 
   method {:extern} new_cell<V>()
-  returns (linear lcell: LinearCell<V>, glinear cellContents: CellContents<V>)
-  ensures cellContents == CellContents(lcell, None)
+  returns (linear lcell: LinearCell<V>, glinear cellContents: LCellContents<V>)
+  ensures cellContents == LCellContents(lcell, None)
 
-  method {:extern} read_lcell<V>(shared lcell: LinearCell<V>, gshared cellContents: CellContents<V>)
+  method {:extern} read_lcell<V>(shared lcell: LinearCell<V>, gshared cellContents: LCellContents<V>)
   returns (shared v: V)
   requires cellContents.lcell == lcell
   requires cellContents.v.Some?
   ensures cellContents.v.value == v
 
-  method {:extern} take_lcell<V>(shared lcell: LinearCell<V>, glinear cellContents: CellContents<V>)
-  returns (linear v: V, glinear cellContents': CellContents<V>)
+  method {:extern} take_lcell<V>(shared lcell: LinearCell<V>, glinear cellContents: LCellContents<V>)
+  returns (linear v: V, glinear cellContents': LCellContents<V>)
   requires cellContents.lcell == lcell
   requires cellContents.v.Some?
   ensures cellContents.v.value == v
   ensures cellContents'.lcell == lcell
   ensures cellContents'.v == None
 
-  method {:extern} give_lcell<V>(shared lcell: LinearCell<V>, glinear cellContents: CellContents<V>, linear v: V)
-  returns (glinear cellContents': CellContents<V>)
+  method {:extern} give_lcell<V>(shared lcell: LinearCell<V>, glinear cellContents: LCellContents<V>, linear v: V)
+  returns (glinear cellContents': LCellContents<V>)
   requires cellContents.lcell == lcell
   requires cellContents.v.None?
   ensures cellContents'.lcell == lcell
